Updated

art/chap11.v
@@ -1,3 +1,13 @@
+(* Chapter 11 * A Case Study *) 
+
+
+
+
+
+(* 11.1 Binary Search Tree *) 
+
+
+(* 11.1.1 The Data Structure *) 
 
 Require Import ZArith Arith. 
 Open Scope Z_scope. 
@@ -18,12 +28,15 @@ Definition Figure_11_1 :=
         Z_leaf
         (Z_bnode 27 Z_leaf Z_leaf))) . 
 
+(* Values tccuring in a Tree *) 
+
 Inductive occ (n:Z) : Z_btree -> Prop := 
     | occ_root  : forall t1 t2,   occ n (Z_bnode n t1 t2)
     | occ_l     : forall p t1 t2, occ n t1 -> occ n (Z_bnode p t1 t2)
     | occ_r     : forall p t1 t2, occ n t2 -> occ n (Z_bnode p t1 t2) . 
 
 
+(* 11.1.2 A Naive Approach to Deciding Occurrence *) 
 Require Import Lia. 
 
 Definition naive_occ_dec : forall n t, {occ n t} + {~ occ n t} . 
@@ -42,6 +55,7 @@ Require Import Extraction.
 
 Extraction naive_occ_dec. 
 
+(* 11.1.3 Describing Search Trees *) 
 
 Inductive min (n:Z) (t:Z_btree) : Prop := 
     | min_intro : (forall p, occ p t -> n < p) -> min n t.
@@ -52,7 +66,8 @@ Inductive maj (n:Z) (t:Z_btree) : Prop :=
 Inductive search_tree : Z_btree -> Prop :=
     | leaf_search_tree : search_tree Z_leaf 
     | bnode_search_tree : forall n t1 t2, 
-            search_tree t1 -> search_tree t2 -> maj n t1 -> min n t2 -> search_tree (Z_bnode n t1 t2) . 
+            search_tree t1 -> search_tree t2 -> maj n t1 -> min n t2 -> 
+            search_tree (Z_bnode n t1 t2) . 
 
 
 
@@ -65,6 +80,7 @@ Inductive min' n : Z_btree -> Prop :=
 Inductive maj' n : Z_btree -> Prop := 
     | max_intro_leaf : maj' n Z_leaf 
     | max_intro_node : forall z t1 t2, maj' n t2 -> z < n -> maj' n (Z_bnode z t1 t2). 
+
 
 Inductive search_tree' : Z_btree -> Prop := 
     | leaf_search_tree' : search_tree' Z_leaf 
@@ -120,15 +136,33 @@ Proof.
 Qed. 
 (* end ex 11.1 *) 
 
+
+
+
+
+
+(* 11.2 Specifying Programs *) 
+
+
+(* 11.2.1 Finding an Occurence *) 
 Definition occ_dec_spec p t : Set := 
     search_tree t -> {occ p t} + { ~ occ p t} . 
 
-Inductive INSERT n t t' : Prop := 
-    insert_intro : (forall p, occ p t  -> occ p t'      ) -> occ n t' -> 
-                   (forall p, occ p t' -> occ p t \/ n=p) -> search_tree t' -> INSERT n t t'. 
 
+(* 11.2.2 Inserting a Number *) 
+
+(* A Predicate for Insertion *) 
+Inductive INSERT n t t' : Prop := 
+    insert_intro : 
+      (forall p, occ p t  -> occ p t'      ) -> occ n t' -> 
+      (forall p, occ p t' -> occ p t \/ n=p) -> search_tree t' -> INSERT n t t'. 
+
+(* 11.2.2.1 The Specification for Insertion *) 
 Definition insert_spec n t : Set := search_tree t -> { t' : Z_btree | INSERT n t t' } . 
 
+
+
+(* 11.2.3 Removing a Number *) 
 Inductive RM n t t' : Prop := 
     rm_intro : 
         ~ occ n t' -> 
@@ -142,4 +176,296 @@ Definition rm_spec n t : Set := search_tree t -> { t' : Z_btree | RM n t t' } .
 
 
 
+(* ex.11.2 *) 
+Definition bin_search_tree  := sig search_tree. 
+
+Definition bin_search_occ   n (t:bin_search_tree) := 
+    match t with 
+    | exist _ t _ => occ n t end. 
+
+Definition bin_search_occ_dec n t := 
+      {bin_search_occ n t} + { ~ bin_search_occ n t }. 
+
+Inductive bin_search_INSERT n t t' : Prop :=
+    bs_insert_intro : 
+      (forall p, bin_search_occ p t -> bin_search_occ p t')  -> 
+      bin_search_occ n t' -> 
+      (forall p, bin_search_occ p t'-> bin_search_occ p t\/n=p) -> 
+      bin_search_INSERT n t t'. 
+
+Definition bin_search_insert_spec n t := { t' | bin_search_INSERT n t t' }. 
+
+Inductive bin_search_RM n t t': Prop := 
+    bs_rm_intro :
+      ~ bin_search_occ n t' -> 
+      (forall p, bin_search_occ p t' -> bin_search_occ p t) -> 
+      (forall p, bin_search_occ p t  -> bin_search_occ p t \/ n=p) -> 
+      bin_search_RM n t t'. 
+
+Definition bin_search_rm_spec n t := { t' | bin_search_RM n t t' }. 
+(* end 11.2 *) 
+
+
+
+
+
+
+
+
+(* 11.3 Auxiliary Lemmas *) 
+
+Lemma not_left : 
+  forall n l r , search_tree (Z_bnode n l r) -> forall p, p>=n -> ~ occ p l. 
+Proof. 
+  red. intros. inversion H.  
+  subst. inversion H7.  
+  now set (H2 p H1). 
+Qed. 
+Reset not_left. 
+
+(* 11.4 Realizing Specifications *) 
+
+(* 11.4.1 Realizing the Occurence Test *) 
+
+Definition occ_dec := forall p t, occ_dec_spec p t.
+Reset occ_dec. 
+
+Lemma min_leaf : forall z, min z Z_leaf. 
+Proof. intros. constructor. inversion 1. Qed.    
+
+Lemma maj_leaf : forall z, maj z Z_leaf. 
+Proof. intros. constructor. inversion 1. Qed.    
+
+Lemma maj_not_occ : forall z t, maj z t -> ~ occ z t. 
+Proof. red. intros. inversion H. set (H1 z H0). lia. Qed.  
+
+Lemma min_not_occ : forall z t, min z t -> ~ occ z t. 
+Proof. red. intros. inversion H. set (H1 z H0). lia. Qed.  
+
+Hint Resolve 
+  insert_intro
+  occ_root occ_l occ_r 
+  min_leaf maj_leaf maj_not_occ min_not_occ : searchtrees. 
+
+Section search_tree_basic_properties. 
+  Variable n:Z.
+  Variable l r : Z_btree. 
+  Hypothesis se : search_tree (Z_bnode n l r). 
+
+  Lemma search_tree_l : search_tree l. 
+  Proof. inversion se. assumption. Qed.   
+  Lemma search_tree_r : search_tree r. 
+  Proof. inversion se. assumption. Qed.   
+  Lemma maj_l : maj n l. 
+  Proof. inversion se. assumption. Qed. 
+  Lemma min_r : min n r. 
+  Proof. inversion se. assumption. Qed. 
+  Lemma not_right : forall p, p<=n -> ~ occ p r. 
+  Proof. inversion se. inversion H5. red. intros. set (H6 p H8). lia. Qed.      
+  Lemma not_left  : forall p, p>=n -> ~ occ p l. 
+  Proof. inversion se. inversion H4. red. intros. set (H6 p H8). lia. Qed.   
+  Lemma go_left : forall p, occ p(Z_bnode n l r) -> p < n -> occ p l. 
+  Proof. intros. inversion se. inversion H; subst; 
+         [ | | inversion H7; set (H1 p H9) ]; auto; lia. Qed. 
+  Lemma go_right : forall p, occ p(Z_bnode n l r) -> p > n -> occ p r.   
+  Proof. intros. inversion se. inversion H; subst; 
+         [ | inversion H6; set(H1 p H9) | ]; auto; lia.  Qed. 
+End search_tree_basic_properties. 
+         
+Hint Resolve go_left go_right not_left not_right
+    search_tree_l search_tree_r maj_l min_r : searchtrees. 
+
+
+Check Z_le_gt_dec. 
+Check Z_le_lt_eq_dec. 
+
+Definition occ_dec : forall p t, occ_dec_spec p t. 
+Proof. 
+  refine 
+  (fix occ_dec p t {struct t} := 
+    match t with 
+    | Z_leaf        => fun h => right _ _ 
+    | Z_bnode n l r => fun h => match Z_le_gt_dec p n with 
+                                | left  h1 => match Z_le_lt_eq_dec p n h1 with 
+                                              | left h'1 => match occ_dec p l _ with 
+                                                            | left  h''1 => left  _ _ 
+                                                            | right h''2 => right _ _ end
+                                              | right h'2=> left _ _  end 
+                                | right h2 => match occ_dec p r _ with 
+                                              | left  h''1  => left  _ _ 
+                                              | right h''2  => right _ _  end end end); 
+                                              subst; eauto with searchtrees. 
+Defined. 
+  
+Extraction occ_dec. 
+
+
+
+
+(* 11.4.2 Insertion *) 
+
+Lemma insert_leaf : forall n, INSERT n Z_leaf (Z_bnode n Z_leaf Z_leaf). 
+Proof. intros. constructor.    
+  - inversion 1. 
+  - constructor.  
+  - inversion 1; tauto.  
+  - repeat constructor; inversion 1. 
+Qed. 
+
+Lemma insert_l : forall n p l l' r, n < p -> search_tree (Z_bnode p l r) -> 
+    INSERT n l l' -> 
+    INSERT n (Z_bnode p l r) (Z_bnode p l' r). 
+Proof. 
+  inversion 3; constructor; intros.  
+  - inversion H6; subst; eauto with searchtrees. 
+  -                      eauto with searchtrees.  
+  - inversion H6; subst; eauto with searchtrees. 
+    + destruct (H4 p0);  eauto with searchtrees. 
+  - inversion H0; subst; constructor; eauto with searchtrees. 
+    + constructor; inversion H11; intros; destruct(H4 p0 H7); 
+      subst; eauto with searchtrees.
+Qed. 
+
+Lemma insert_r : forall n p l r r', n > p -> search_tree (Z_bnode p l r) -> 
+    INSERT n r r' -> 
+    INSERT n (Z_bnode p l r) (Z_bnode p l r') . 
+Proof. 
+  inversion 3; constructor; intros. 
+  - inversion H6; subst; eauto with searchtrees. 
+  - eauto with searchtrees. 
+  - inversion H6; subst; eauto with searchtrees. 
+    + destruct (H4 p0); eauto with searchtrees. 
+  - inversion H0; subst; constructor; eauto with searchtrees. 
+    + constructor; inversion H12; intros; destruct(H4 p0 H7);
+      subst; eauto with searchtrees; lia.  
+Qed. 
+
+Lemma insert_eq : forall n l r, search_tree (Z_bnode n l r) -> 
+      INSERT n (Z_bnode n l r) (Z_bnode n l r). 
+Proof. constructor; eauto with searchtrees. Qed.  
+
+Hint Resolve insert_leaf insert_l insert_r insert_eq : searchtrees. 
+
+
+
+(* Should There be a Test function for search_tree ? *)
+
+Definition insert : forall n t, insert_spec n t. 
+Proof. 
+  refine 
+  (fix insert n t :=
+    match t with 
+    | Z_leaf        => fun s => exist _ (Z_bnode n Z_leaf Z_leaf) _ 
+    | Z_bnode p l r => fun s => 
+        match Z_le_gt_dec n p with 
+        | left  Hle => match Z_le_lt_eq_dec n p Hle with 
+                       | left  Heq => match insert n l _ with 
+                                      | exist _ l' _ => exist _ (Z_bnode p l' r) _ end 
+                       | right Hlt => exist _ (Z_bnode n l r) _ end 
+        | right Hgt => match insert n r _ with
+                       | exist _ r' _ => exist _ (Z_bnode p l r') _ end end end ); 
+                       subst; eauto with searchtrees.  
+Defined.  
+
+
+
+
+Require Import List. 
+Import ListNotations. 
+
+Definition list2tree_spec l := 
+  { t | search_tree t /\ (forall p, In p l <-> occ p t)}. 
+
+
+Definition list2tree_aux_spec l t := 
+  search_tree t -> 
+  { t' | search_tree t' /\ (forall p, In p l \/ occ p t <-> occ p t') }.  
+
+Definition list2tree_aux : forall l t, list2tree_aux_spec l t. 
+Proof.   
+  refine
+    (fix list2tree_aux l t := 
+         match l with 
+         | []     => fun s => exist _ t _
+         | p::l'  => fun s => 
+             match insert p t s with
+             | exist _ t' _ => match list2tree_aux l' t' _ with
+                               | exist _ t'' _ => exist _ t'' _ end end end).
+  - split; auto.
+    + split; auto.
+      * intuition. inversion H0. 
+  - case i; auto.
+  - case a; auto.
+    intros; split; auto.
+    intros; case a; intros; split; auto.
+    + destruct 1 as [H3 | H3].
+      * { destruct H3; intros; subst. 
+        - destruct (H2 p0). apply H3. right. case i; auto.          
+        - destruct (H2 p0). auto. }   
+      * { destruct (H2 p0). apply H4. right. case i; auto. }  
+    + intros. 
+      destruct a       as [H4 H5]. 
+      destruct (H5 p0) as [H6 H7]. 
+      destruct (H7 H3).
+      * left. cbn. right. assumption.     
+      * destruct i.    
+        destruct (H11 p0 H8); auto.  
+        cbn. left. left. assumption.     
+Defined. 
+
+Definition list2tree : forall l, list2tree_spec l. 
+Proof. 
+  refine ( fun l => 
+    match list2tree_aux l Z_leaf _ with 
+    | exist _ t _ => exist _ t _  end ). 
+  - constructor.  
+  - destruct a as [H1 H2].  
+    split; auto. 
+    + intros p. destruct (H2 p); split. 
+      * intros. apply H. left. assumption.    
+      * intros. 
+        { destruct (H0 H3). 
+        - auto. 
+        - inversion H4. } 
+Defined. 
+
+
+(* Extracted Programs *) 
+
+Extraction insert .
+Extraction list2tree_aux . 
+Extraction list2tree . 
+
+
+
+
+
+
+(* 11.4.3 Removing Elements *) 
+
+Inductive RMAX t t' n : Prop :=
+  rmax_intro : occ n t -> 
+               (forall p, occ p t -> p<=n) -> 
+               (forall q, occ q t' -> occ q t) -> 
+               (forall q, occ q t -> occ q t' \/ q = n) -> 
+               ~ occ n t' -> search_tree t' -> RMAX t t' n. 
+
+Definition rmax_sig t q := {t' | RMAX t t' q}. 
+(*
+Definition is_bnode t := match t with 
+                         | Z_leaf => False
+   | _      => True end . *)
+Inductive is_bnode : Z_btree -> Prop := 
+  is_bnode_intro : forall n l r, is_bnode (Z_bnode n l r). 
+
+Definition rmax_spec t  := search_tree t -> is_bnode t -> {q & rmax_sig t q} . 
+
+
+
+(* 11.5 Possible Improvements *) 
+
+(* 11.6 Another Example *)
+
+(* ==> see Monin's book[66] chapter 12 *) 
+(*     "Undeerstanding Formal Methods" 2002 *) 
 
