art/chap12.v
@@ -854,4 +854,3 @@ Module Type LSORT.
 End LSORT. 
 
 
-
